src/tls/Epochs.fst
@@ -30,7 +30,7 @@ module MR = FStar.Monotonic.RRef
 module MS = FStar.Monotonic.Seq
 type random = TLSInfo.random 
 
-inline_for_extraction let epochs_debug = true
+(* debug printing *)
 val discard: bool -> ST unit
   (requires (fun _ -> True))
   (ensures (fun h0 _ h1 -> h0 == h1))
@@ -39,7 +39,7 @@ let print s = discard (IO.debug_print_string ("EPO| "^s^"\n"))
 unfold val trace: s:string -> ST unit
   (requires (fun _ -> True))
   (ensures (fun h0 _ h1 -> h0 == h1))
-unfold let trace = if epochs_debug then print else (fun _ -> ())
+unfold let trace = if Flags.debug_Epochs then print else (fun _ -> ())
 
 
 type epoch_region_inv (#i:id) (hs_rgn:rgn) (r:reader (peerId i)) (w:writer i) =
